Refactor and extend OPML to Kore (semantics WIP)

kore/src/Substitution.v
@@ -1,3 +1,278 @@
 From Kore Require Export Syntax.
 
 Import Kore.Syntax.Notations.
+
+Section Substitution.
+  Context {Σ : Signature}.
+  Open Scope kore_scope.
+
+  Fixpoint bevar_subst (ps : Pattern) (x : nat)
+    (p : Pattern) : Pattern :=
+  match p with
+   | kore_top _ | kore_bot _ | kore_fevar _ | kore_fsvar _ | kore_bsvar _ => p
+   | kore_bevar n =>
+     match compare_nat n x with
+     | Nat_less _ _ _ => kore_bevar n
+     | Nat_equal _ _ _ => ps
+     | _ => kore_bevar n (* kore_bevar (Nat.pred n) *)
+     end
+   | kore_not φ  => kore_not (bevar_subst ps x φ)
+   | kore_imp φ1 φ2  => kore_imp (bevar_subst ps x φ1) (bevar_subst ps x φ2)
+   | kore_iff φ1 φ2  => kore_iff (bevar_subst ps x φ1) (bevar_subst ps x φ2)
+   | kore_and φ1 φ2  => kore_and (bevar_subst ps x φ1) (bevar_subst ps x φ2)
+   | kore_or φ1 φ2   => kore_or (bevar_subst ps x φ1) (bevar_subst ps x φ2)
+   | kore_app σ args => kore_app σ (map (bevar_subst ps x) args)
+   | kore_exists s φ => kore_exists s (bevar_subst ps (S x) φ)
+   | kore_forall s φ => kore_forall s (bevar_subst ps (S x) φ)
+   | kore_mu s φ     => kore_mu s (bevar_subst ps x φ)
+   | kore_nu s φ     => kore_nu s (bevar_subst ps x φ)
+   | kore_ceil s1 s2 φ => kore_ceil s1 s2 (bevar_subst ps x φ)
+   | kore_floor s1 s2 φ => kore_floor s1 s2 (bevar_subst ps x φ)
+   | kore_equals s1 s2 φ1 φ2 => kore_equals s1 s2 (bevar_subst ps x φ1) (bevar_subst ps x φ2)
+   | kore_in s1 s2 φ1 φ2 => kore_in s1 s2 (bevar_subst ps x φ1) (bevar_subst ps x φ2)
+  end.
+
+  Fixpoint bsvar_subst (ps : Pattern) (x : nat)
+    (p : Pattern) : Pattern :=
+  match p with
+   | kore_top _ | kore_bot _ | kore_fevar _ | kore_fsvar _ | kore_bevar _ => p
+   | kore_bsvar n =>
+     match compare_nat n x with
+     | Nat_less _ _ _ => kore_bsvar n
+     | Nat_equal _ _ _ => ps
+     | _ => kore_bsvar n (* kore_bsvar (Nat.pred n) *)
+     end
+   | kore_not φ  => kore_not (bsvar_subst ps x φ)
+   | kore_imp φ1 φ2  => kore_imp (bsvar_subst ps x φ1) (bsvar_subst ps x φ2)
+   | kore_iff φ1 φ2  => kore_iff (bsvar_subst ps x φ1) (bsvar_subst ps x φ2)
+   | kore_and φ1 φ2  => kore_and (bsvar_subst ps x φ1) (bsvar_subst ps x φ2)
+   | kore_or φ1 φ2   => kore_or (bsvar_subst ps x φ1) (bsvar_subst ps x φ2)
+   | kore_app σ args => kore_app σ (map (bsvar_subst ps x) args)
+   | kore_exists s φ => kore_exists s (bsvar_subst ps x φ)
+   | kore_forall s φ => kore_forall s (bsvar_subst ps x φ)
+   | kore_mu s φ     => kore_mu s (bsvar_subst ps (S x) φ)
+   | kore_nu s φ     => kore_nu s (bsvar_subst ps (S x) φ)
+   | kore_ceil s1 s2 φ => kore_ceil s1 s2 (bsvar_subst ps x φ)
+   | kore_floor s1 s2 φ => kore_floor s1 s2 (bsvar_subst ps x φ)
+   | kore_equals s1 s2 φ1 φ2 => kore_equals s1 s2 (bsvar_subst ps x φ1) (bsvar_subst ps x φ2)
+   | kore_in s1 s2 φ1 φ2 => kore_in s1 s2 (bsvar_subst ps x φ1) (bsvar_subst ps x φ2)
+  end.
+
+End Substitution.
+
+Module Notations.
+
+  Notation "p '^[' 'evar:' x ↦ t ']'" :=
+    (bevar_subst t x p) : kore_scope.
+  Notation "p '^[' 'svar:' x ↦ t ']'" :=
+    (bsvar_subst t x p) : kore_scope.
+
+End Notations.
+
+Section Substitution.
+  Import Notations.
+  Open Scope kore_scope.
+
+  Context {Σ : Signature}.
+
+  Lemma bevar_subst_opml_size :
+    forall φ x n,
+      pat_size (bevar_subst (kore_fevar x) n φ) = pat_size φ.
+  Proof.
+    induction φ using Pat_ind; simpl; intros; try reflexivity.
+    all: try by erewrite ->IHφ1, ->IHφ2.
+    all: try by erewrite ->IHφ.
+    * by case_match.
+    * f_equal. induction H; simpl.
+      reflexivity.
+      rewrite IHForall.
+      erewrite H.
+      reflexivity.
+  Defined.
+
+  Lemma bsvar_subst_opml_size :
+    forall φ X n,
+      pat_size (bsvar_subst (kore_fsvar X) n φ) = pat_size φ.
+  Proof.
+    induction φ using Pat_ind; simpl; intros; try reflexivity.
+    all: try by erewrite ->IHφ1, ->IHφ2.
+    all: try by erewrite ->IHφ.
+    * by case_match.
+    * f_equal. induction H; simpl.
+      reflexivity.
+      rewrite IHForall.
+      erewrite H.
+      reflexivity.
+  Defined.
+
+  Lemma well_sorted_bevar_subst :
+    forall φ ψ s s' fe fs n,
+    well_sorted fe fs s φ ->
+    well_sorted default default s' ψ ->
+    fe n = Some s' ->
+    well_sorted (update n None fe) fs s (φ^[evar: n ↦ ψ]).
+  Proof.
+    induction φ using Pat_ind; intros; simpl in *; trivial.
+    * case_match; simpl.
+      - destruct decide in H. 2: by simpl in H.
+        unfold update.
+        destruct decide.
+        + lia.
+        + simpl. rewrite e.
+          rewrite decide_eq_same. reflexivity.
+      - subst. rewrite H1 in H.
+        destruct decide. 2: by simpl in H.
+        inversion e. subst.
+        eapply well_sorted_weaken. 3: eassumption.
+        apply default_is_strongest.
+        apply default_is_strongest.
+      - destruct decide. 2: by simpl in H.
+        unfold update.
+        destruct decide.
+        + lia.
+        + simpl. rewrite e.
+          rewrite decide_eq_same. reflexivity.
+    * apply andb_split_1 in H0 as WF1. rewrite WF1.
+      clear WF1. simpl.
+      apply andb_split_2 in H0.
+      {
+        remember (arg_sorts σ) as xs.
+        clear Heqxs. generalize dependent xs.
+        induction H; simpl; intros. assumption.
+        case_match.
+        - congruence.
+        - apply andb_split_1 in H3 as H31.
+          apply andb_split_2 in H3.
+          erewrite H, IHForall; try eassumption.
+          reflexivity.
+      }
+    * erewrite IHφ; try by eassumption.
+      reflexivity.
+    * erewrite IHφ1, IHφ2; try by eassumption.
+      reflexivity.
+      by apply andb_split_2 in H.
+      by apply andb_split_1 in H.
+    * erewrite IHφ1, IHφ2; try by eassumption.
+      reflexivity.
+      by apply andb_split_2 in H.
+      by apply andb_split_1 in H.
+    * erewrite IHφ1, IHφ2; try by eassumption.
+      reflexivity.
+      by apply andb_split_2 in H.
+      by apply andb_split_1 in H.
+    * erewrite IHφ1, IHφ2; try by eassumption.
+      reflexivity.
+      by apply andb_split_2 in H.
+      by apply andb_split_1 in H.
+    * simpl in *.
+      rewrite shift_update.
+      erewrite IHφ; try by eauto.
+    * simpl in *.
+      rewrite shift_update.
+      erewrite IHφ; try by eauto.
+    * simpl in *.
+      erewrite IHφ; try by eauto.
+    * simpl in *.
+      erewrite IHφ; try by eauto.
+    * erewrite IHφ; try by eassumption.
+      by apply andb_split_2 in H.
+      by apply andb_split_1 in H.
+    * erewrite IHφ; try by eassumption.
+      by apply andb_split_2 in H.
+      by apply andb_split_1 in H.
+    * erewrite IHφ1, IHφ2; try by eassumption.
+        by apply andb_split_2 in H.
+        by apply andb_split_1, andb_split_2 in H.
+        by apply andb_split_1, andb_split_1 in H.
+    * erewrite IHφ1, IHφ2; try by eassumption.
+        by apply andb_split_2 in H.
+        by apply andb_split_1, andb_split_2 in H.
+        by apply andb_split_1, andb_split_1 in H.
+  Defined.
+
+  Lemma well_sorted_bsvar_subst :
+    forall φ ψ s s' fe fs n,
+    well_sorted fe fs s φ ->
+    well_sorted default default s' ψ ->
+    fs n = Some s' ->
+    well_sorted fe (update n None fs) s (φ^[svar: n ↦ ψ]).
+  Proof.
+    induction φ using Pat_ind; intros; simpl in *; trivial.
+    * case_match; simpl.
+      - destruct decide in H. 2: by simpl in H.
+        unfold update.
+        destruct decide.
+        + lia.
+        + simpl. rewrite e.
+          rewrite decide_eq_same. reflexivity.
+      - subst. rewrite H1 in H.
+        destruct decide. 2: by simpl in H.
+        inversion e. subst.
+        eapply well_sorted_weaken. 3: eassumption.
+        apply default_is_strongest.
+        apply default_is_strongest.
+      - destruct decide. 2: by simpl in H.
+        unfold update.
+        destruct decide.
+        + lia.
+        + simpl. rewrite e.
+          rewrite decide_eq_same. reflexivity.
+    * apply andb_split_1 in H0 as WF1. rewrite WF1.
+      clear WF1. simpl.
+      apply andb_split_2 in H0.
+      {
+        remember (arg_sorts σ) as xs.
+        clear Heqxs. generalize dependent xs.
+        induction H; simpl; intros. assumption.
+        case_match.
+        - congruence.
+        - apply andb_split_1 in H3 as H31.
+          apply andb_split_2 in H3.
+          erewrite H, IHForall; try eassumption.
+          reflexivity.
+      }
+    * erewrite IHφ; try by eassumption.
+      reflexivity.
+    * erewrite IHφ1, IHφ2; try by eassumption.
+      reflexivity.
+      by apply andb_split_2 in H.
+      by apply andb_split_1 in H.
+    * erewrite IHφ1, IHφ2; try by eassumption.
+      reflexivity.
+      by apply andb_split_2 in H.
+      by apply andb_split_1 in H.
+    * erewrite IHφ1, IHφ2; try by eassumption.
+      reflexivity.
+      by apply andb_split_2 in H.
+      by apply andb_split_1 in H.
+    * erewrite IHφ1, IHφ2; try by eassumption.
+      reflexivity.
+      by apply andb_split_2 in H.
+      by apply andb_split_1 in H.
+    * simpl in *.
+      erewrite IHφ; try by eauto.
+    * simpl in *.
+      erewrite IHφ; try by eauto.
+    * simpl in *.
+      rewrite shift_update.
+      erewrite IHφ; try by eauto.
+    * simpl in *.
+      rewrite shift_update.
+      erewrite IHφ; try by eauto.
+    * erewrite IHφ; try by eassumption.
+      by apply andb_split_2 in H.
+      by apply andb_split_1 in H.
+    * erewrite IHφ; try by eassumption.
+      by apply andb_split_2 in H.
+      by apply andb_split_1 in H.
+    * erewrite IHφ1, IHφ2; try by eassumption.
+        by apply andb_split_2 in H.
+        by apply andb_split_1, andb_split_2 in H.
+        by apply andb_split_1, andb_split_1 in H.
+    * erewrite IHφ1, IHφ2; try by eassumption.
+        by apply andb_split_2 in H.
+        by apply andb_split_1, andb_split_2 in H.
+        by apply andb_split_1, andb_split_1 in H.
+  Defined.
+
+End Substitution.
