kore/src/Freshness.v
@@ -1,0 +1,71 @@
+From Kore Require Export Syntax.
+
+Section Freshness.
+
+  Context {Σ : Signature}.
+
+  Fixpoint free_evars (φ : Pattern) {struct φ} : gset evar :=
+  match φ with
+   | kore_fevar x => {[x]}
+   | kore_imp φ1 φ2 | kore_iff φ1 φ2
+   | kore_and φ1 φ2 | kore_or φ1 φ2
+   | kore_equals _ _ φ1 φ2 | kore_in _ _ φ1 φ2
+      => free_evars φ1 ∪ free_evars φ2
+   | kore_app σ args
+      => foldr (fun x acc => free_evars x ∪ acc) ∅ args
+   | kore_exists _ φ | kore_forall _ φ
+   | kore_mu _ φ | kore_nu _ φ 
+   | kore_not φ | kore_ceil _ _ φ | kore_floor _ _ φ
+      => free_evars φ
+   | kore_bevar _ | kore_fsvar _ | kore_bsvar _
+   | kore_bot _ | kore_top _ => ∅
+  end.
+
+  Fixpoint free_svars (φ : Pattern) {struct φ} : gset svar :=
+  match φ with
+   | kore_fsvar X => {[X]}
+   | kore_imp φ1 φ2 | kore_iff φ1 φ2
+   | kore_and φ1 φ2 | kore_or φ1 φ2
+   | kore_equals _ _ φ1 φ2 | kore_in _ _ φ1 φ2
+      => free_svars φ1 ∪ free_svars φ2
+   | kore_app σ args
+      => foldr (fun x acc => free_svars x ∪ acc) ∅ args
+   | kore_exists _ φ | kore_forall _ φ
+   | kore_mu _ φ | kore_nu _ φ 
+   | kore_not φ | kore_ceil _ _ φ | kore_floor _ _ φ
+      => free_svars φ
+   | kore_bevar _ | kore_fevar _ | kore_bsvar _
+   | kore_bot _ | kore_top _ => ∅
+  end.
+
+  Fixpoint dep_filter {A} (f : A -> bool) (l : list A) {struct l} :
+    list {a : A & f a} :=
+  match l with
+    | [] => []
+    | x::xs =>
+      (if f x as b0 return f x = b0 -> list {a : A & f a}
+      then fun P => existT x P :: dep_filter f xs
+      else fun P => dep_filter f xs
+      ) eq_refl
+  end.
+
+
+  Definition fresh_evar (s : sort) (φ : Pattern) : 
+    { x : evar & decide (evar_sort x = s) }.
+  Proof.
+    pose (elements (free_evars φ)) as fs.
+    pose (dep_filter (fun x => decide (evar_sort x = s)) fs) as filtered.
+    simpl in filtered.
+    exact (fresh filtered).
+  Defined.
+  Definition fresh_svar (s : sort) (φ : Pattern) :
+    { x : svar & decide (svar_sort x = s) }.
+  Proof.
+    pose (elements (free_svars φ)) as fs.
+    pose (dep_filter (fun x => decide (svar_sort x = s)) fs) as filtered.
+    simpl in filtered.
+    exact (fresh filtered).
+  Defined.
+
+
+End Freshness.
