kore/src/Semantics.v
@@ -1,0 +1,261 @@
+From Equations Require Import Equations.
+From Kore Require Export Substitution
+                         Basics.
+Require Import Coq.Program.Equality.
+
+
+
+Section Semantics.
+  Context {Σ : Signature}.
+
+  Record OPMLModel := {
+    carrier :> sort -> Set;
+    app (σ : symbol) :
+       @hlist _ carrier (arg_sorts σ) -> propset (carrier (ret_sort σ));
+    inhabited (s : sort) : Inhabited (carrier s)
+  }.
+
+  Section with_model.
+
+  Context {M : OPMLModel}.
+  Record Valuation : Type := {
+    evar_valuation (x : evar) : carrier M (evar_sort x);
+    svar_valuation (X : svar) : propset (carrier M (svar_sort X)) ;
+  }.
+
+  Definition app_ext
+    (σ : symbol)
+    (args : @hlist _ (fun s => propset (carrier M s)) (arg_sorts σ))
+    : propset (carrier M (ret_sort σ)) :=
+  PropSet (
+    fun e => exists (l : @hlist _ (carrier M) (arg_sorts σ)),
+      pointwise_elem_of _ l args /\ e ∈ app M σ l
+  ).
+
+  Fixpoint map_to_hlist {A} (F : A -> Type) (f : forall (a : A), F a) (l : list A) {struct l} : @hlist Type id (map F l) :=
+    match l return @hlist _ _ (map F l) with
+    | []    => hnil
+    | x::xs => hcons (f x) (map_to_hlist F f xs)
+    end.
+  Print map_to_hlist.
+
+  Fixpoint app_map (l : list Pattern)
+    {ls}
+    (pf : app_ws (well_sorted default default) l ls)
+    (f : forall (φ :Pattern) {s}
+         (pf : well_sorted default default s φ)
+         (psize : pat_size φ < 1 + foldr (fun φ acc => pat_size φ + acc) 0 l), propset (carrier M s)) {struct l} :
+    @hlist _ (fun x => propset (carrier M x)) ls
+    .
+  Proof.
+    (* refine (
+    match l return  -> @hlist _ (fun x => propset (carrier M x)) ls with
+    | []    => _
+    | x::xs => _
+    end eq_refl
+    ). *)
+    clear app_map.
+    revert ls f pf.
+    induction l; intros.
+    * (* nil *)
+      simpl in *.
+      destruct ls.
+      - exact hnil.
+      - congruence.
+    * (* cons *)
+      simpl in *.
+      destruct ls.
+      - congruence.
+      - apply andb_split_1 in pf as pf1.
+        apply andb_split_2 in pf as pf2.
+        apply hcons.
+        + eapply f.
+          exact pf1.
+          lia.
+        + apply IHl.
+          ** intros. eapply f. exact pf0. lia.
+          ** assumption.
+  Defined.
+
+  Program Definition update_evar_val
+    (ev : evar)
+    (x : carrier M (evar_sort ev))
+    (val : Valuation) : Valuation :=
+    {|
+    evar_valuation := fun ev' : evar => _;
+      (* if decide (ev = ev')
+      then x
+      else evar_valuation val ev' ; *)
+    svar_valuation := (svar_valuation val)
+    |}.
+  Next Obligation.
+    intros ev H ρ ev'.
+    destruct (decide (ev = ev')).
+    * rewrite -e. exact H.
+    * exact (evar_valuation ρ ev').
+  Defined.
+
+  Program Definition update_svar_val
+    (sv : svar)
+    (X : propset (carrier M (svar_sort sv)))
+    (val : Valuation) : Valuation :=
+    {|
+    evar_valuation := (evar_valuation val);
+    svar_valuation := fun sv' : svar =>
+      if decide (sv = sv') is left _ then _ else svar_valuation val sv' ;
+    |}.
+  Next Obligation.
+    intros.
+    rewrite -wildcard'.
+    exact X.
+  Defined.
+
+  (* Oké-e ha a nem well-sorted dolgoknak valami default értéket
+     adjunk, és így elhagyjuk a well-sorted judgementet (Hws-t) *)
+  Equations? eval (ρ : Valuation) (φ : Pattern) {s}
+    (Hws : well_sorted default default s φ)
+      : propset (carrier M s) by wf (pat_size φ) :=
+    eval ρ (kore_fevar x) pf    := _ ;
+    eval ρ (kore_fsvar X) pf    := _;
+    eval ρ (kore_bevar x) pf    := ∅ ;
+    eval ρ (kore_bsvar x) pf    := ∅ ;
+
+    eval ρ (kore_app σ args) pf := _;
+
+    eval ρ (kore_bot s0)   pf    := ∅ ;
+    eval ρ (kore_top s0)   pf    := ⊤ ;
+    eval ρ (kore_not φ)   pf    := (⊤ ∖ eval ρ φ _);
+    eval ρ (kore_imp φ1 φ2)  pf := (⊤ ∖ (eval ρ φ1 _)) ∪ (eval ρ φ2 _);
+    eval ρ (kore_iff φ1 φ2)  pf := _;
+    eval ρ (kore_and φ1 φ2)  pf := _;
+    eval ρ (kore_or φ1 φ2)  pf := _;
+
+    eval ρ (kore_exists s0 φ)    pf := _;
+    eval ρ (kore_forall s0 φ)    pf := _;
+    eval ρ (kore_mu s0 φ)    pf := _;
+    eval ρ (kore_nu s0 φ)    pf := _;
+
+    eval ρ (kore_ceil s1 s2 φ) pf := _;
+    eval ρ (kore_floor s1 s2 φ) pf := _;
+    eval ρ (kore_equals s1 s2 φ1 φ2) pf := _;
+    eval ρ (kore_in s1 s2 φ1 φ2) pf := _;.
+    Proof.
+      * (* kore_fevar *)
+        simpl in *.
+        epose {[ evar_valuation ρ x ]} as d.
+        exact d.
+        Unshelve.
+        destruct decide.
+        - rewrite e. typeclasses eauto.
+        - simpl in pf. congruence.
+      * (* kore_fsvar *)
+        simpl in *.
+        epose (svar_valuation ρ X) as d.
+        destruct decide.
+        - rewrite <- e. exact d.
+        - simpl in pf. congruence.
+      * (* kore_app *)
+        apply andb_split_1 in pf as pf1.
+        apply andb_split_2 in pf as pf2.
+        pose (app_ext σ (app_map args pf2 (eval ρ))) as X.
+        destruct decide.
+        rewrite e. exact X.
+        inversion pf1.
+      * (* kore_imp *)
+        by apply andb_split_1 in pf.
+      * lia.
+      * (* kore_imp *)
+        by apply andb_split_2 in pf.
+      * lia.
+      * (* kore_eq *)
+        apply andb_split_1 in pf as pf1.
+        apply andb_split_1 in pf1 as pf0.
+        apply andb_split_2 in pf1 as pf2. clear pf1.
+        rename pf0 into pf1.
+        apply andb_split_2 in pf as pf3. clear pf.
+        destruct decide. 2: { simpl in *. congruence. }
+        epose (X1 := eval ρ φ1 s1 pf1 _).
+        epose (X2 := eval ρ φ2 s1 pf2 _).
+        exact (PropSet (fun e => X1 = X2)).
+        Unshelve.
+        all: lia.
+      * (* kore_ex *)
+        eapply (propset_fa_union (
+          fun c : carrier M s0 =>
+            let newx := fresh_evar s0 φ in
+            eval (update_evar_val (projT1 newx) _ ρ)
+                      (bevar_subst (kore_fevar (projT1 newx)) 0 φ)
+                      _ _ _
+        )).
+        Unshelve.
+        - pose proof (projT2 newx) as Is. simpl in Is.
+          destruct decide. 2: simpl in Is; congruence.
+          rewrite e. exact c.
+        - eapply (well_sorted_bevar_subst _ (kore_fevar (projT1 newx)) s s0 _ _ 0) in pf.
+          3: reflexivity.
+          2: { cbn. exact (projT2 newx). }
+          clear -pf.
+          assert (update 0 None (shift default (Some s0)) = default). {
+            unfold update, shift.
+            extensionality x. destruct x; simpl.
+            reflexivity.
+            reflexivity.
+          }
+          rewrite H in pf.
+          exact pf.
+        - rewrite bevar_subst_size. lia.
+      * (* kore_mu *)
+        exact ∅.
+    Defined.
+  Print eval.
+
+  Definition satM φ s (ws : well_sorted default default s φ) :=
+    forall ρ, eval ρ φ ws = ⊤.
+  Definition Theory := propset Pattern.
+    (* dependent pairs are not well-supported by stdpp *)
+  Definition satT (Γ : Theory) :=
+    forall p, p ∈ Γ ->
+      exists s, { pf : well_sorted default default s p & satM p s pf }.
+
+  Import PropExtensionality.
+  #[export]
+  Instance propset_leibniz_equiv A : LeibnizEquiv (propset A).
+  Proof.
+    intros x y H. unfold equiv in H. unfold set_equiv_instance in H.
+    destruct x,y.
+    apply f_equal. apply functional_extensionality.
+    intros x. apply propositional_extensionality.
+    specialize (H x). destruct H as [H1 H2].
+    split; auto.
+  Qed.
+
+  Fixpoint HForall {J} {A : J -> Type}
+    (P : ∀ j, A j -> Prop)
+    {js : list J} (v : @hlist J A js) {struct v} : Prop :=
+    match v with
+    | hnil => True
+    | hcons x xs => P _ x ∧ HForall P xs
+    end.
+
+  Fixpoint HBiForall {J1 J2} {A1 : J1 -> Type} {A2 : J2 -> Type}
+    (P : ∀ j1 j2, A1 j1 -> A2 j2 -> Prop)
+    {js1 : list J1}
+    {js2 : list J2}
+    (v1 : @hlist J1 A1 js1) (v2 : @hlist J2 A2 js2)
+      {struct v1} : Prop :=
+    match v1, v2 with
+    | hnil, hnil => True
+    | hcons x xs, hcons y ys => P _ _ x y ∧ HBiForall P xs ys
+    | _, _ => False
+    end.
+
+  Fixpoint hmap {J} {A B : J -> Type}
+    (f : ∀ j, A j -> B j)
+    {js : list J} (v : @hlist J A js) : @hlist J B js :=
+  match v with
+  | hnil => hnil
+  | hcons x xs => hcons (f _ x) (hmap f xs)
+  end.
+
+End with_model.
+End Semantics.
